more cleanup; move some more lemmas from UnsaturatedSolinas to own files or Util

src/Bedrock/UnsaturatedSolinas.v
@@ -1,5 +1,4 @@
 Require Import Coq.ZArith.ZArith.
-Require Import Coq.derive.Derive.
 Require Import Coq.Strings.String.
 Require Import Coq.micromega.Lia.
 Require Import coqutil.Word.Interface.
@@ -23,6 +22,7 @@ Require Import Crypto.Bedrock.Types.
 Require Import Crypto.Bedrock.MakeAccessSizes.
 Require Import Crypto.Bedrock.MakeNames.
 Require Import Crypto.Bedrock.MakeListLengths.
+Require Import Crypto.Bedrock.MaxBounds.
 Require Import Crypto.Bedrock.Util.
 Require Import Crypto.Bedrock.VarnameGenerator.
 Require Import Crypto.Bedrock.Proofs.Func.
@@ -30,12 +30,7 @@ Require Import Crypto.Bedrock.Translation.Func.
 Require Import Crypto.COperationSpecifications.
 Require Import Crypto.PushButtonSynthesis.UnsaturatedSolinas.
 Require Import Crypto.Util.ListUtil.
-Require Import Crypto.Util.ZRange.BasicLemmas.
 Require Import Crypto.Util.ZUtil.Modulo.
-Require Import Crypto.Util.Tactics.BreakMatch.
-Require Import Crypto.Util.ZUtil.Tactics.LtbToLt.
-Require Import Crypto.Util.ZUtil.Tactics.RewriteModSmall.
-Require Import Crypto.Util.ZUtil.Tactics.PullPush.Modulo.
 Require Import Crypto.Language.API.
 Require Import Coq.Lists.List. (* after SeparationLogic *)
 
@@ -84,11 +79,6 @@ Section __.
     : bedrock_func :=
     ("carry_mul", make_bedrock_func res).
 
-  Definition max_range : ZRange.zrange :=
-    {|ZRange.lower:=0; ZRange.upper:=2^Semantics.width-1|}.
-  Definition max_bounds : list (option ZRange.zrange) :=
-    repeat (Some max_range) n.
-
   Section Proofs.
     Context {ok : Types.ok}.
     Existing Instance semantics_ok.
@@ -108,24 +98,26 @@ Section __.
       as a precondition. *)
       (loose_bounds_ok :
          ZRange.type.option.is_tighter_than
-           (t:=type_listZ) (Some loose_bounds) (Some max_bounds) = true)
+           (t:=type_listZ) (Some loose_bounds)
+           (Some (max_bounds n)) = true)
       (check_args_ok :
          check_args n s c Semantics.width (ErrorT.Success tt)
          = ErrorT.Success tt).
 
-    Context (inname_gen_varname_gen_ok :
-               forall n m, inname_gen n <> varname_gen m)
-            (outname_gen_varname_gen_ok :
-               forall n m, outname_gen n <> varname_gen m)
-            (outname_gen_inname_gen_ok :
-               forall n m, outname_gen n <> inname_gen m).
-    Context (inname_gen_unique :
-               forall i j : nat, inname_gen i = inname_gen j <-> i = j)
-            (outname_gen_unique :
-               forall i j : nat, outname_gen i = outname_gen j <-> i = j).
+    Context (inname_gen_varname_gen_ok : disjoint inname_gen varname_gen)
+            (outname_gen_varname_gen_ok : disjoint outname_gen varname_gen)
+            (outname_gen_inname_gen_ok : disjoint outname_gen inname_gen).
+    Context (inname_gen_unique : unique inname_gen)
+            (outname_gen_unique : unique outname_gen).
 
-    Definition Bignum :=
+    Definition Bignum : Semantics.word -> list Semantics.word -> Semantics.mem -> Prop :=
       array scalar (word.of_Z word_size_in_bytes).
+
+    Definition BignumSuchThat
+               (addr : Semantics.word) (ws : list Semantics.word) (P: list Z -> Prop)
+      : Semantics.mem -> Prop :=
+      let xs := map word.unsigned ws in
+      sep (emp (P xs)) (Bignum addr ws).
 
     Lemma Bignum_of_bytes addr bs :
       length bs = (n * Z.to_nat word_size_in_bytes)%nat ->
@@ -136,84 +128,16 @@ Section __.
     Admitted. (* TODO *)
 
     Lemma Bignum_to_bytes addr x :
-      list_Z_bounded_by max_bounds (map word.unsigned x) ->
+      list_Z_bounded_by (max_bounds n) (map word.unsigned x) ->
       Lift1Prop.iff1
         (Bignum addr x)
         (array ptsto (word.of_Z 1) addr (encode_bytes x)).
     Admitted. (* TODO *)
 
-    (* TODO: clean up and move *)
-    Lemma relax_list_Z_bounded_by r1 r2 x :
-      ZRange.type.option.is_tighter_than
-        (t:=type_listZ) (Some r1) (Some r2) = true ->
-      list_Z_bounded_by r1 x ->
-      list_Z_bounded_by r2 x.
-    Proof.
-      cbn in r1, r2 |- *. intros.
-      pose proof length_list_Z_bounded_by _ x ltac:(eassumption).
-      match goal with H : FoldBool.fold_andb_map _ _ _ = true |- _ =>
-                      pose proof H;
-                        apply FoldBool.fold_andb_map_length in H
-      end.
-      generalize dependent r1; generalize dependent r2.
-      generalize dependent x; induction x; cbn [length].
-      { destruct r2; cbn [length]; intros; [ | lia].
-        reflexivity. }
-      { destruct r1, r2; cbn [length]; intros; try lia; [ ].
-        cbv [list_Z_bounded_by] in *. cbn [FoldBool.fold_andb_map] in *.
-        repeat match goal with
-               | _ => progress cleanup
-               | H : _ && _ = true |- _ =>
-                 apply Bool.andb_true_iff in H
-               end.
-        apply Bool.andb_true_iff; split.
-        { break_innermost_match; [ | reflexivity].
-          break_innermost_match_hyps; [ | congruence ].
-          cbv [ZRange.is_tighter_than_bool] in *.
-          repeat match goal with
-                 | _ => progress cleanup
-                 | H : _ && _ = true |- _ =>
-                   apply Bool.andb_true_iff in H
-                 end.
-          apply Bool.andb_true_iff; split; Z.ltb_to_lt; lia. }
-        { eapply IHx;
-            match goal with
-            | |- length _ = length _ =>
-              idtac (* no eassumption on length goals *)
-            | _ => try eassumption
-            end; lia. } }
-    Qed.
-
     Lemma relax_to_max_bounds x :
       list_Z_bounded_by loose_bounds x ->
-      list_Z_bounded_by max_bounds x.
+      list_Z_bounded_by (max_bounds n) x.
     Proof. apply relax_list_Z_bounded_by; auto. Qed.
-
-    (* TODO: maybe upstream? *)
-    Lemma list_Z_bounded_by_Forall x r m :
-      list_Z_bounded_by (repeat (Some r) m) x ->
-      Forall (fun z : Z => ZRange.lower r <= z <= ZRange.upper r) x.
-    Proof.
-      intros.
-      pose proof length_list_Z_bounded_by _ x ltac:(eassumption).
-      cbv [list_Z_bounded_by] in *.
-      rewrite repeat_length in *.
-      generalize dependent x.
-      generalize dependent m.
-      induction m; intros;
-        destruct x; intros; cbn [length] in *; subst;
-          try lia; [ | ]; constructor;
-            [ | apply IHm; [ | lia] ].
-      all: cbn [repeat FoldBool.fold_andb_map] in *.
-      all: repeat match goal with
-               | _ => progress cleanup
-               | _ => progress Z.ltb_to_lt
-               | H : _ && _ = true |- _ =>
-                 apply Bool.andb_true_iff in H
-               | _ => solve [auto]
-               | _ => lia
-               end.
-    Qed.
 
     Lemma bounded_by_loose_bounds_length x :
       list_Z_bounded_by loose_bounds x -> length x = n.
@@ -222,91 +146,15 @@ Section __.
       rewrite length_loose_bounds in *. lia.
     Qed.
 
-    Lemma max_bounds_range_iff x :
-      let bytes := (Memory.bytes_per
-                      (width:=Semantics.width) access_size.word) in
-      list_Z_bounded_by max_bounds x <->
-      (length x = n /\
-       Forall
-        (fun z : Z =>
-           0 <= z < 2 ^ (Z.of_nat bytes * 8)) x).
-   Proof.
-     cbv [max_bounds max_range list_Z_bounded_by].
-     rewrite bits_per_word_eq_width by auto using width_0mod_8.
-     generalize n as m.
-     induction x; destruct m; split;
-       cbn [FoldBool.fold_andb_map repeat]; try congruence; intros;
-         repeat match goal with
-                | _ => progress cleanup
-                | _ => progress cbn [length ZRange.lower ZRange.upper] in *
-                | |- Forall _ [] => solve [constructor]
-                | |- Forall _ (_ :: _) => constructor
-                | H: Forall _ (_ :: _) |- _ =>
-                  inversion H; clear H; subst
-                | |- (_ && _)%bool = true =>
-                  apply Bool.andb_true_iff; split
-                | H: (_ && _)%bool = true |- _ =>
-                  apply Bool.andb_true_iff in H; destruct H
-                | H : context [iff] |- _ => eapply H; solve [eauto]
-                | H : context [iff] |- _ =>
-                  rewrite H; auto; congruence
-                | |- _ /\ _ => split
-                | |- S _ = S _ => f_equal
-                | _ => progress Z.ltb_to_lt
-                | _ => congruence
-                | _ => lia
-                end.
-   Qed.
-
-    Lemma map_word_wrap_bounded' r x m :
-      ZRange.is_tighter_than_bool r max_range = true ->
-      list_Z_bounded_by (repeat (Some r) m) x ->
-      map word.wrap x = x.
-    Proof.
-      intros.
-      pose proof length_list_Z_bounded_by _ x ltac:(eassumption).
-      cbv [max_bounds max_range list_Z_bounded_by
-                      ZRange.is_tighter_than_bool] in *.
-      rewrite repeat_length in *.
-      generalize dependent m.
-      generalize dependent x; induction x; destruct m;
-        repeat match goal with
-               | _ => progress intros
-               | _ => progress cleanup
-               | _ => progress
-                        cbn [length FoldBool.fold_andb_map
-                                    ZRange.upper ZRange.lower
-                                    repeat map] in *
-               | H : _ && _ = true |- _ =>
-                 apply Bool.andb_true_iff in H
-               | IH : context [map word.wrap ?x = ?x] |- _ =>
-                 rewrite IH with (m:=m) by (try eassumption; lia)
-               | _ => progress Z.ltb_to_lt
-               | |- word.wrap ?x :: ?y = ?x :: ?y =>
-                 cbv [word.wrap]; Z.rewrite_mod_small;
-                   reflexivity
-               | _ => congruence
-               end.
-    Qed.
-
-    Lemma map_word_wrap_bounded x :
-      list_Z_bounded_by max_bounds x ->
-      map word.wrap x = x.
-    Proof.
-      intros. eapply map_word_wrap_bounded'; [ | eassumption ].
-      apply ZRange.is_tighter_than_bool_Reflexive.
-    Qed.
-
     Ltac crush_list_ptr_subgoals :=
       repeat match goal with
              | _ => progress cbv [WeakestPrecondition.literal]
              | _ => rewrite word.of_Z_unsigned
              | _ => rewrite map.get_put_diff by congruence
              | _ => rewrite map.get_put_same by auto
-             | |- WeakestPrecondition.get _ _ _ =>
-               eexists
-             | _ => apply max_bounds_range_iff;
-                    solve [auto using relax_to_max_bounds]
+             | |- WeakestPrecondition.get _ _ _ => eexists
+             | _ => eapply max_bounds_range_iff;
+                    solve [auto using relax_to_max_bounds, relax_correct]
              | _ => solve [apply word.unsigned_range]
              | _ => solve [auto using eval_bytes_range]
              | _ => reflexivity
@@ -317,7 +165,6 @@ Section __.
              [ solve [crush_list_ptr_subgoals] .. | ];
              eexists; sepsimpl;
              [ solve [crush_list_ptr_subgoals] .. | ].
-
     Ltac next_argument :=
       (exists 1%nat); sepsimpl; cbn [firstn skipn];
       [ solve [eauto using firstn_length_le] | ].
@@ -342,28 +189,19 @@ Section __.
       fun functions =>
         forall wx wy px py pout wold_out t m
                (Ra Rr : Semantics.mem -> Prop),
-          let x := map word.unsigned wx in
-          let y := map word.unsigned wy in
-          (* these bounds go here instead of within Solinas_carry_mul_correct
-             because they are needed to prove the length of the output *)
-          list_Z_bounded_by loose_bounds x ->
-          list_Z_bounded_by loose_bounds y ->
-          length wold_out = n ->
-          sep (sep (Bignum px wx) (Bignum py wy)) Ra m ->
-          sep (Bignum pout wold_out) Rr m ->
+          sep (sep (BignumSuchThat px wx (list_Z_bounded_by loose_bounds))
+                   (BignumSuchThat py wy (list_Z_bounded_by loose_bounds))) Ra m ->
+          sep (BignumSuchThat pout wold_out (fun l => length l = n)) Rr m ->
+          let post := Solinas_carry_mul_correct (map word.unsigned wx)
+                                                (map word.unsigned wy) in
           WeakestPrecondition.call
             functions name t m
             (px :: py :: pout :: nil)
             (fun t' m' rets =>
                t = t' /\
                rets = []%list /\
-               Lift1Prop.ex1
-                 (fun wout =>
-                    let out := map word.unsigned wout in
-                    sep
-                      (sep
-                         (emp (Solinas_carry_mul_correct x y out))
-                         (Bignum pout wout)) Rr) m').
+               exists wout,
+                 sep (BignumSuchThat pout wout post) Rr m').
 
     Lemma carry_mul_correct carry_mul_name:
       forall carry_mul_res :
@@ -377,6 +215,7 @@ Section __.
             ((carry_mul_name, make_bedrock_func carry_mul_res) :: functions).
     Proof.
       cbv [spec_of_carry_mul make_bedrock_func]; intros.
+      cbv [BignumSuchThat] in *. sepsimpl.
 
       (* get the carry_mul correctness proof *)
       match goal with H : _ = ErrorT.Success _ |- _ =>
@@ -411,8 +250,8 @@ Section __.
         sepsimpl_hyps; ssplit; [ congruence | congruence | eexists ].
         fold Bignum in *.
         sepsimpl;
-          [ rewrite map_unsigned_of_Z, map_word_wrap_bounded
-            by (apply max_bounds_range_iff; eauto);
+          [ erewrite map_unsigned_of_Z, map_word_wrap_bounded
+            by (eapply max_bounds_range_iff; eauto);
             match goal with H : _ |- _ => apply H; assumption end | ].
         subst. cbv [Bignum expr.Interp].
         match goal with
@@ -457,14 +296,14 @@ Section __.
         cbn - [Memory.bytes_per]; tauto. }
       { (* input access sizes are accurate *)
         cbn - [Memory.bytes_per]; ssplit; try tauto;
-          apply max_bounds_range_iff;
+          eapply max_bounds_range_iff;
             auto using relax_to_max_bounds. }
       { (* output access sizes are legal *)
         pose proof bits_per_word_le_width.
         cbn - [Memory.bytes_per]; tauto. }
       { (* output access sizes are accurate *)
         cbn - [Memory.bytes_per].
-        apply max_bounds_range_iff;
+        eapply max_bounds_range_iff;
           apply relax_to_max_bounds, relax_correct.
         match goal with H : _ |- _ => apply H end. }
       { (* space is reserved for output lists *)
@@ -484,11 +323,11 @@ Section __.
                end.
         cbn [Compilers.base_interp] in *.
         exists (map word.unsigned wold_out).
-        sepsimpl; [ rewrite map_length; congruence | ].
+        sepsimpl; [ rewrite map_length in *; congruence | ].
         exists pout; sepsimpl; [ ].
         match goal with
           H : Solinas_carry_mul_correct _ _ ?e |- _ =>
-          assert (list_Z_bounded_by max_bounds e)
+          assert (list_Z_bounded_by (max_bounds n) e)
             by (apply relax_to_max_bounds, relax_correct; apply H)
         end.
         eexists.
